Superposition_Calculus/Grounded_First_Order_Superposition.thy
@@ -27,7 +27,8 @@ locale grounded_first_order_superposition_calculus =
 begin
 
 (* TODO: Write about this limitation of locales! *)
-interpretation nonground_typing typeof_fun "UNIV :: 'v set".
+interpretation nonground_typing typeof_fun "UNIV :: 'v set"
+  by unfold_locales (rule infinite_UNIV)
 
 sublocale ground: ground_superposition_calculus where
   less\<^sub>t = "(\<prec>\<^sub>t\<^sub>G)" and select = select\<^sub>G
@@ -264,7 +265,8 @@ end
 context first_order_superposition_calculus
 begin
 
-interpretation nonground_typing typeof_fun "UNIV :: 'v set".
+interpretation nonground_typing typeof_fun "UNIV :: 'v set"
+  by unfold_locales (rule infinite_UNIV)
 
 sublocale
   lifting_intersection
