Superposition_Calculus/Nonground_Term.thy
@@ -20,19 +20,6 @@ type_synonym 'f ground_term = "'f gterm"
 notation subst_apply_term (infixl "\<cdot>t" 67)
 notation subst_compose (infixl "\<odot>" 75)
 
-lemma infinite_terms: "infinite (UNIV :: ('f, 'v) term set)"
-proof-
-  have "infinite (UNIV :: ('f, 'v) term list set)"
-    using infinite_UNIV_listI.
-
-  then have "\<And>f :: 'f. infinite ((Fun f) ` (UNIV :: ('f, 'v) term list set))"
-    by (meson finite_imageD injI term.inject(2))
-
-  then show "infinite (UNIV :: ('f, 'v) term set)"
-    using infinite_super top_greatest by blast
-qed
-
-
 subsection\<open>Unified naming\<close>
 
 locale vars_def =
@@ -61,6 +48,18 @@ global_interpretation "term": grounding_def where
   to_ground_def = gterm_of_term and from_ground_def = term_of_gterm .
 
 subsection\<open>Term\<close>
+
+lemma infinite_terms: "infinite (UNIV :: ('f, 'v) term set)"
+proof-
+  have "infinite (UNIV :: ('f, 'v) term list set)"
+    using infinite_UNIV_listI.
+
+  then have "\<And>f :: 'f. infinite ((Fun f) ` (UNIV :: ('f, 'v) term list set))"
+    by (meson finite_imageD injI term.inject(2))
+
+  then show "infinite (UNIV :: ('f, 'v) term set)"
+    using infinite_super top_greatest by blast
+qed
 
 lemma renaming_vars_term:
   assumes "\<forall>x. is_Var (\<rho> x)"
