Superposition_Calculus/Renaming.thy
@@ -4,61 +4,7 @@ theory Renaming
     Nonground_Clause
 begin
 
-section \<open>Abstract Renaming\<close>
-
-locale renaming =
-  fixes variables :: "'v set"
-  assumes infinite_variables: "infinite variables"
-begin
-
-
-(* TODO: generalize? *)
-lemma renaming_exists: 
-  assumes
-    "X \<subseteq> variables"
-    "Y \<subseteq> variables"
-    "finite X"
-    "finite Y"
-  obtains \<rho>\<^sub>1 \<rho>\<^sub>2 :: "('f, 'v) subst" where
-    "term_subst.is_renaming \<rho>\<^sub>1" 
-    "term_subst.is_renaming \<rho>\<^sub>2"
-    "\<rho>\<^sub>1 ` X \<inter> \<rho>\<^sub>2 ` Y = {}"
-proof-
-  let ?newVars = "variables - Y"
-
-  have "infinite ?newVars"
-    by (simp add: assms(4) infinite_variables)
-
-  then obtain renaming where 
-    renaming: "inj renaming" "renaming ` X \<subseteq> ?newVars"
-    using obtain_inj_endo[OF assms(3)]
-    by blast
-
-   define \<rho>\<^sub>1 :: "('f, 'v) subst" where 
-    \<rho>\<^sub>1: "\<rho>\<^sub>1  = (\<lambda>var. Var (renaming var))"
-
-  have "inj \<rho>\<^sub>1" "(\<forall>x. is_Var (\<rho>\<^sub>1 x))"
-    unfolding \<rho>\<^sub>1
-    using renaming(1)
-    by (simp_all add: inj_on_def)
-    
-  then have "term_subst.is_renaming \<rho>\<^sub>1"
-    by (simp add: term_subst_is_renaming_iff)
-
-  moreover have "term_subst.is_renaming Var"
-    by simp
-
-  moreover have "\<rho>\<^sub>1 ` X \<inter>  Var ` Y = {}"
-    using \<rho>\<^sub>1 renaming(2) by auto
-
-  ultimately show ?thesis  
-    using that
-    by blast
-qed
-
-end
-
-
+(* TODO Martin: Where should we put this?  *)
 section \<open>Renamings as Bijections on Natural Numbers\<close>
 
 text \<open>Renamings can be defined as bijections between variables; They then become invertible (both
